verif/btrees/verif_getrecord.v
@@ -1,0 +1,86 @@
+(** * verif_getrecord.v : Correctness proof of RL_GetRecord  *)
+
+Require Import VST.floyd.proofauto.
+Require Import VST.floyd.library.
+Require Import relation_mem.
+Instance CompSpecs : compspecs. make_compspecs prog. Defined.
+Definition Vprog : varspecs. mk_varspecs prog. Defined.
+
+Require Import VST.msl.wand_frame.
+Require Import VST.msl.iter_sepcon.
+Require Import VST.floyd.reassoc_seq.
+Require Import VST.floyd.field_at_wand.
+Require Import FunInd.
+Require Import btrees.
+Require Import btrees_sep.
+Require Import btrees_spec.
+Require Import verif_entryindex.
+Require Import verif_currnode.
+Require Import verif_isvalid.
+Require Import index.
+
+Lemma body_RL_GetRecord: semax_body Vprog Gprog f_RL_GetRecord RL_GetRecord_spec.
+Proof.
+  start_function.
+  destruct r as [root prel].
+  pose (r:=(root,prel)).
+  destruct c as [|[n i] c'].
+  { destruct H; inv H; inv H2. }
+  pose (c:=(n,i)::c').
+  forward_call(r,c,pc,numrec).  (* t'1=isValid(cursor) *)
+  { unfold r. unfold c. cancel. }
+  forward_if (PROP () LOCAL (temp _cursor pc) SEP (relation_rep (root, prel) numrec; cursor_rep ((n, i) :: c') (root, prel) pc)).
+  - forward.                    (* skip *)
+    unfold r. unfold c. entailer!.
+  - assert_PROP(False). fold c r in H1. rewrite H1 in H4. simpl in H4. inv H4. contradiction.
+  - forward_call(r,c,pc,numrec). (* t'2=entryIndex(cursor) *)
+    { fold r c. cancel. }
+    forward_call(r,c,pc,numrec). (* t'3=currnode(cursor) *)
+    unfold c. simpl.
+    assert(SUBNODE: subnode n root).
+    { destruct H. apply complete_cursor_subnode in H. simpl in H. auto. }
+    assert(SUBREP: subnode n root) by auto. apply subnode_rep in SUBREP.
+    rewrite SUBREP.
+    destruct n as [ptr0 le isLeaf First Last pn].
+    pose (n:=btnode val ptr0 le isLeaf First Last pn). fold n.
+    rewrite unfold_btnode_rep with (n:=n) at 1. unfold n.
+    Intros ent_end.
+    forward.                    (* t'7=t'3->numKeys *)
+    gather_SEP 2 3 4 5. replace_SEP 0 (btnode_rep n).
+    { entailer!. rewrite unfold_btnode_rep. unfold n. Exists ent_end. entailer!. }
+    gather_SEP 0 3. replace_SEP 0 (btnode_rep root).
+    { entailer!. unfold n. apply wand_frame_elim. }
+    gather_SEP 0 1 2. replace_SEP 0 (relation_rep r numrec).
+    { entailer!. } deadvars!. simpl numKeys. fold n. fold n in c. fold c.
+    pose (normc := match index_eqb i (ip (numKeys n)) with
+                   | true => moveToNext c r
+                   | false => c
+                   end).
+    forward_if(PROP ( )
+     LOCAL (temp _t'7 (Vint (Int.repr (Z.of_nat (numKeys_le le))));
+     temp _t'2 (Vint (Int.repr (rep_index i))); temp _cursor pc)
+     SEP (relation_rep r numrec; cursor_rep normc r pc; emp)).
+    { forward_call(c,pc,r,numrec).
+      entailer!. unfold normc. simpl.
+      apply (f_equal Int.signed) in H4.
+      unfold root_wf, node_wf, n in H2. apply H2 in SUBNODE. simpl in SUBNODE.
+      rewrite Int.signed_repr in H4.
+      rewrite Int.signed_repr in H4.
+      destruct i as [|ii]. simpl in H4. omega.
+      simpl in H4. apply Nat2Z.inj in H4. subst. simpl.
+      rewrite Nat.eqb_refl. cancel.
+      rep_omega. destruct H. apply complete_correct_rel_index in H.
+      destruct i. simpl. rep_omega. simpl in H. simpl. rep_omega. }
+    { forward.                  (* skip *)
+      entailer!. unfold normc.
+      admit. }
+    forward_call(r,normc,pc,numrec). (* t'4=currnode(cursor) *)
+    split. right. admit. auto.
+    forward_call(r,normc,pc,numrec). (* t'5=entryIndex(cursor) *)
+    split. right. admit. auto.
+    unfold relation_rep. unfold r.
+    rewrite SUBREP. fold n. rewrite unfold_btnode_rep with (n:=n) at 1. unfold n.
+    autorewrite with norm.
+    (* Intros ent_end. *)
+    admit.
+Admitted.
